{
 "cells": [
  {
   "cell_type": "markdown",
   "id": "e9d7d048-b2a1-4346-8582-e26fba90e03a",
   "metadata": {},
   "source": [
    "# Derivatives of 1D functions\n",
    "\n",
    "A review of differentiation learned at school\n",
    "\n",
    "This time with some proofs ..."
   ]
  },
  {
   "cell_type": "markdown",
   "id": "a817d59d-a206-4548-a656-1f7fea616c5f",
   "metadata": {},
   "source": [
    "# Difference Quotient\n",
    "\n",
    "The definition of the difference quotient is fundamental to the definition of the differential of a function.\n",
    "\n",
    "Let $f(x)$ denote some univariate function and assume that it is a real valued function.\n",
    "\n",
    "The difference quotient is defined as the ratio:\n",
    "\n",
    "$$\n",
    "D_f(x) = \\frac{f(x) - f(x_0)}{x -x_0}\n",
    "$$\n",
    "\n",
    "At a point $x_0 + e$ in the interval $x_0 \\le x_0 + e \\le x$ the slope of the tangent to the function equals the difference quotient.\n",
    "\n",
    "The slope or differential quotient of the tangent is denoted $f'(x_0 + e)$ . In the limit $x \\to x_0$ the quantity $e$ approaches $0$ and the difference quotient $D_f(x)$ approaches the derivative $f'(x_0)$ of function $f(x)$.\n",
    "\n",
    "Some useful relations are provided here:\n",
    "\n",
    "$$\n",
    "f(x) = f(x_0) - (x - x_0) \\cdot D_f(x) = f(x_0) - (x - x_0) \\cdot f'(x_0 + e)\n",
    "$$\n",
    "\n",
    "$$\n",
    "\\lim_{x \\to x_0} D_f(x) = f'(x_0)\n",
    "$$\n",
    "\n",
    "----\n"
   ]
  },
  {
   "cell_type": "markdown",
   "id": "a8869e9e-2200-43c8-abbf-2ef2d8887f23",
   "metadata": {},
   "source": [
    "# Rules for Diffentiation\n",
    "\n",
    "It is assumed that all function can be differentiated in the vicinity of $x_0$.\n",
    "\n",
    "## Differentiation of a sum of two functions\n",
    "\n",
    "Define function $f(x)$ as the sum of functions $f_1(x)$ and $f_2(x)$:\n",
    "\n",
    "$$\\begin{gather}\n",
    "f(x) = f(x_0) + (x - x_0) \\cdot f'(x_0 + e) \\\\\n",
    "f(x) = f_1(x_0) + f_2(x_0) + (x - x_0) \\cdot \\left[f_1'(x_0 + e_1)  f_2'(x_0 + e_1) \\right] \\\\\n",
    "f'(x_0 + e) = f_1'(x_0 + e_1)  f_2'(x_0 + e_1)  \\\\\n",
    "\\ \\\\\n",
    "x \\to x_0;\\ e,\\ e_1,\\ e_2 \\to 0 \\\\\n",
    "f'(x_0) = f_1'(x_0) + f_2'(x_0)\n",
    "\\end{gather}\n",
    "$$\n",
    "\n",
    "## Differentiation of a product of two function\n",
    "\n",
    "Define function $f(x)$ as the product of functions $f_1(x)$ and $f_2(x)$:\n",
    "\n",
    "$$\n",
    "f(x) = f_1(x) \\cdot f_2{x}\n",
    "$$\n",
    "\n",
    "$$\\begin{gather}\n",
    "f(x) = f(x_0) + (x - x_0) \\cdot f'(x_0 + e) \\\\\n",
    "f(x) = f_1(x) \\cdot f_2(x) = \\left(f_1(x_0) + (x - x_0) \\cdot f_1'(x_0 + e_1) \\right) \\cdot \\left(f_2(x_0) + (x - x_0) \\cdot f_2'(x_0 + e_2) \\right) \\\\\n",
    "f(x) = f_1(x_0) \\cdot f_2(x_0) + (x - x_0) \\cdot \\left( f_1'(x_0  + e_1) \\cdot f_2(x_0) + f_1(x_0) \\cdot f_2'(x_0 + e_2) \\right) \\\\\n",
    "f'(x_0 + e)= f_1'(x_0  + e_1) \\cdot f_2(x_0) + f_1(x_0) \\cdot f_2'(x_0 + e_2) \\\\\n",
    "\\ \\\\\n",
    "x \\to x_0;\\ e,\\ e_1,\\ e_2 \\to 0 \\\\\n",
    "f'(x_0) = f_1'(x_0) \\cdot f_2(x_0) + f_1(x_0) \\cdot f_2'(x_0)\n",
    "\\end{gather}\n",
    "$$\n",
    "\n",
    "## Differentiation of the reciprocal of a function\n",
    "\n",
    "Define function $f(x)$ as the reciprocal of function $f_1(x)$:\n",
    "\n",
    "$$\n",
    "f(x) = \\frac{1}{f_1(x)}\n",
    "$$\n",
    "\n",
    "$$\\begin{gather}\n",
    "f(x) = f(x_0) + (x - x_0) \\cdot f'(x_0 + e) \\\\\n",
    "\\frac{1}{f_1(x)} - \\frac{1}{f_1(x_0)}  = -\\frac{f_1(x) - f_1(x_0)}{f_1(x) \\cdot f_1(x_0)} = (x - x_0) \\cdot f'(x_0 + e) \\\\\n",
    "-\\frac{f_1(x_0) + (x - x_0) \\cdot f_1'(x_0 + e_1) - f_1(x_0)}{f_1(x) \\cdot f_1(x_0)} = (x - x_0) \\cdot f'(x_0 + e) \\\\\n",
    "f'(x_0 + e) = -\\frac{f_1'(x_0 + e_1)}{f_1(x) \\cdot f_1(x_0)} \\\\\n",
    "\\ \\\\\n",
    "x \\to x_0;\\ e,\\ e_1 \\to 0 \\\\\n",
    "f'(x_0) = -\\frac{f_1'(x_0)}{f_1^2(x_0)}\n",
    "\\end{gather}\n",
    "$$\n",
    "\n",
    "## Differentiation of the ratio of two functions\n",
    "\n",
    "Define function $f(x)$ as the ratio of functions $f_1(x)$ and $f_2(x)$:\n",
    "\n",
    "$$\n",
    "f(x) = \\frac{f_1(x)}{f_2(x)}\n",
    "$$\n",
    "\n",
    "By application of the *product rule* we get:\n",
    "\n",
    "$$\\begin{gather}\n",
    "f'(x) = f_1'(x) \\cdot \\frac{1}{f_2(x)} - f_1(x) \\cdot \\frac{f_2'(x)}{f_2^2(x)} \\\\ \n",
    "f'(x) = \\frac{f_1'(x) \\cdot f_2(x) - f_1(x) \\cdot f_2'(x)}{f_2^2(x)}\n",
    "\\end{gather}\n",
    "$$\n",
    "\n",
    "## Differentiation of *concatenated* functions / Chain Rule\n",
    "\n",
    "We define a function $g(y)$ which where $y$ depends on another function $f(x)$. We want to differentiate function $g(f(x))$ with respect to variable $x$.\n",
    "\n",
    "$$\\begin{gather}\n",
    "g(y) = g(y_0) + (y - y_0) \\cdot g'(y_0 + e) \\\\\n",
    "y = f(x) \\\\\n",
    "y_0 = f(x_0) \\\\\n",
    "f(x) = f(x_0) + (x - x_0) \\cdot f'(x_0 + e_1) \\\\\n",
    "g(y) - g(y_0) = \\left(f(x_0) + (x - x_0) \\cdot f'(x_0 + e_1) - f(x_0) \\right) \\cdot g'(y_0 + e) \\\\\n",
    "g(y) - g(y_0) = (x - x_0) \\cdot f'(x_0 + e_1) \\cdot g'(y_0 + e) \\\\\n",
    "\\frac{g(y) - g(y_0)}{x - x_0} = f'(x_0 + e_1) \\cdot g'(y_0 + e) \\\\\n",
    "\\ \\\\\n",
    "y \\to y_0;\\ x \\to x_0;\\  e,\\ e_1 \\to 0 \\\\\n",
    "g'(x) = f'(x) \\cdot g'(y) \n",
    "\\end{gather}\n",
    "$$"
   ]
  },
  {
   "cell_type": "markdown",
   "id": "bad63a67-78bb-4139-b04f-64f742479bd7",
   "metadata": {},
   "source": [
    "# Differentiation of frequently used functions\n",
    "\n",
    "Differentiation of $f(x) = x^n$\n",
    "\n",
    "The difference quotient is defined by\n",
    "\n",
    "$$\n",
    "D(x) = \\frac{(x+h)^n - x^n}{h}\n",
    "$$\n",
    "\n",
    "$(x+h)^n$ can be expressed by a binomial series\n",
    "\n",
    "$$\n",
    "D(x) = \\frac{\\sum_{k=0}^n \\binom{n}{k}  x^{(n-k)} \\cdot h^k - x^n}{h} = \\frac{x^n + n \\cdot h \\cdot x^{n-1} + \\sum_{k=2}^n \\binom{n}{k}  x^{(n-k)} \\cdot h^k - x^n}{h} = n \\cdot h \\cdot x^{n-1} + \\sum_{k=2}^n \\binom{n}{k}  x^{(n-k)} h^{k-1}\n",
    "$$\n",
    "\n",
    "In the limit $h \\to 0$ we get:\n",
    "\n",
    "$$\n",
    "f'(x) = n \\cdot h \\cdot x^{n-1}\n",
    "$$"
   ]
  },
  {
   "cell_type": "code",
   "execution_count": null,
   "id": "4284664d-200e-422e-b0ab-0ff7e89511f0",
   "metadata": {},
   "outputs": [],
   "source": []
  }
 ],
 "metadata": {
  "kernelspec": {
   "display_name": "Python 3 (ipykernel)",
   "language": "python",
   "name": "python3"
  },
  "language_info": {
   "codemirror_mode": {
    "name": "ipython",
    "version": 3
   },
   "file_extension": ".py",
   "mimetype": "text/x-python",
   "name": "python",
   "nbconvert_exporter": "python",
   "pygments_lexer": "ipython3",
   "version": "3.11.5"
  }
 },
 "nbformat": 4,
 "nbformat_minor": 5
}
